Update goose examples

src/go_lang/examples/append_log.v
@@ -24,7 +24,7 @@ Definition writeHdr: val :=
     UInt64Put "hdr" (Log.get "sz" "log");;
     UInt64Put (SliceSkip "hdr" #8) (Log.get "sz" "log");;
     disk.Write #0 "hdr".
-Definition writeHdr_t: ⊢ writeHdr : (Log.T -> unitT).
+Theorem writeHdr_t: ⊢ writeHdr : (Log.T -> unitT).
 Proof. typecheck. Qed.
 Hint Resolve writeHdr_t : types.
 
@@ -43,7 +43,7 @@ Definition Init: val :=
       ] in
       writeHdr "log";;
       ("log", #true).
-Definition Init_t: ⊢ Init : (intT -> (Log.T * boolT)).
+Theorem Init_t: ⊢ Init : (intT -> (Log.T * boolT)).
 Proof. typecheck. Qed.
 Hint Resolve Init_t : types.
 
@@ -53,7 +53,7 @@ Definition Get: val :=
     if: "i" < "sz"
     then (disk.Read (#1 + "i"), #true)
     else (slice.nil, #false).
-Definition Get_t: ⊢ Get : (Log.T -> intT -> (blockT * boolT)).
+Theorem Get_t: ⊢ Get : (Log.T -> intT -> (blockT * boolT)).
 Proof. typecheck. Qed.
 Hint Resolve Get_t : types.
 
@@ -65,7 +65,7 @@ Definition writeAll: val :=
       let: "bk" := SliceGet "bks" !"i" in
       disk.Write ("off" + !"i") "bk";;
       Continue.
-Definition writeAll_t: ⊢ writeAll : (slice.T blockT -> intT -> unitT).
+Theorem writeAll_t: ⊢ writeAll : (slice.T blockT -> intT -> unitT).
 Proof. typecheck. Qed.
 Hint Resolve writeAll_t : types.
 
@@ -83,7 +83,7 @@ Definition Append: val :=
       writeHdr "newLog";;
       "log" <- "newLog";;
       #true.
-Definition Append_t: ⊢ Append : (refT Log.T -> slice.T blockT -> boolT).
+Theorem Append_t: ⊢ Append : (refT Log.T -> slice.T blockT -> boolT).
 Proof. typecheck. Qed.
 Hint Resolve Append_t : types.
 
@@ -95,6 +95,6 @@ Definition Reset: val :=
     ] in
     writeHdr "newLog";;
     "log" <- "newLog".
-Definition Reset_t: ⊢ Reset : (refT Log.T -> unitT).
+Theorem Reset_t: ⊢ Reset : (refT Log.T -> unitT).
 Proof. typecheck. Qed.
 Hint Resolve Reset_t : types.
